csci2625
2014.09.02

is Vx(P(x) -> Q(x)) equivalent to (VxP(x)) -> (VxQ(x))

let P(x) = x >= 0
    Q(x) = x <= 0

U = real numbers

Vx(x >= 0 -> x <= 0) ?= (Vx(x >= 0)) -> (Vx(x <= 0))
        false                      true

No, not equivalent.

De Morgan's laws for quantifiers:

    !ExP(x) equivalent to Vx!P(x)
        when true: for every x, P(x) is false
            false: there is an x for which P(x) is true

    !VxP(x) equivalent to Ex!P(x)
        when true: there is an x for which P(x) is false
            false: P(x) true for every x

Example 12
    D(x): "x is in this discrete math class", 
    C(x): "x has taken a course in computer science"

    The premises are Vx(D(x) -> C(x)) and D(Marla). 
    The conclusion is C(Marla).

    1. Vx(D(x) -> C(x))     Premise
    2. D(Marla) -> C(Marla) Universal instantiation from (1)
    3. D(Marla)             Premise
    4. C(Marla)             Modus ponens from (2) and (3)

* Inference rules table and quantified inference rules will be given for test.


